@prefix owl: <http://www.w3.org/2002/07/owl#> .
@prefix rdf: <http://www.w3.org/1999/02/22-rdf-syntax-ns#> .
@prefix skos: <http://www.w3.org/2004/02/skos/core#> .
@prefix eg: <https://example.net/my/minimal/> .
@prefix ext: <https://example.net/my/extension/> .

ext:vocab
    rdf:type skos:ConceptScheme ;
    skos:prefLabel "Simple Vocabulary Extension"@en ;
    skos:definition "This is an example of an extension to an iSamples vocabulary."@en ;
    skos:inScheme eg:vocab ;
.

ext:liquid
    rdf:type skos:Concept ;
    skos:prefLabel "Liquid"@en ;
    skos:definition "A thing that was considered to be of a liquid state at the time of observation. \nThis concept is for demonstration purposes only."@en ;
    skos:inScheme ext:vocab ;
    skos:broader eg:thing ;
.

ext:water
    rdf:type skos:Concept ;
    skos:prefLabel "Water"@en ;
    skos:altLabel "Aqua"@en ;
    skos:altLabel "H2O" ;
    skos:note "This is the first line of a note.\n Here's the second line."@en ;
    skos:note "There may be multiple notes in a concept."@en ;
    skos:definition "A thing that was considered to be liquid water at the time of observation. \nThis concept is for demonstration purposes only."@en ;
    skos:inScheme ext:vocab ;
    skos:broader ext:liquid ;
.
